Minor simplification

pub/stlc_type_equiv.v
@@ -59,7 +59,7 @@ Inductive ty : Type :=
 
 Inductive ty_vl : Type :=
   | TVBool  : ty_vl
-  | TVFun   : ty -> ty -> ty_vl
+  | TVFun   : ty_vl -> ty_vl -> ty_vl
 .
 
 
@@ -88,27 +88,27 @@ Definition tenv := list ty.
 Inductive type_eval : ty -> ty_vl -> Prop :=
 | teval_bool: 
     type_eval TBool TVBool
-| teval_fun: forall T1 T2,
-    type_eval (TFun T1 T2) (TVFun T1 T2)
-| teval_dom: forall TF T1 T2 V1,
-    type_eval TF (TVFun T1 T2) ->
+| teval_fun: forall T1 T2 V1 V2,
+    (* NOTE: there is a choice whether to eval T1,T2
+       here or in type_reify *)
     type_eval T1 V1 ->
-    type_eval (TDom TF) V1
-| teval_img: forall TF T1 T2 V2,
-    type_eval TF (TVFun T1 T2) ->
     type_eval T2 V2 ->
+    type_eval (TFun T1 T2) (TVFun V1 V2)
+| teval_dom: forall TF V1 V2,
+    type_eval TF (TVFun V1 V2) ->
+    type_eval (TDom TF) V1
+| teval_img: forall TF V1 V2,
+    type_eval TF (TVFun V1 V2) ->
     type_eval (TRange TF) V2
 .
 
 Inductive type_reify : ty_vl -> ty -> Prop :=
 | treify_bool: 
     type_reify TVBool TBool
-| treify_fun: forall T1 T2 V1 V2 T1' T2',
-    type_eval T1 V1 ->
-    type_eval T2 V2 ->
+| treify_fun: forall V1 V2 T1' T2',
     type_reify V1 T1' ->
     type_reify V2 T2' ->
-    type_reify (TVFun T1 T2) (TFun T1' T2')
+    type_reify (TVFun V1 V2) (TFun T1' T2')
 .
 
 Definition type_normalize T T': Prop := 
@@ -165,9 +165,9 @@ Proof.
   econstructor. econstructor. econstructor. econstructor.
   simpl. eauto.
   2: econstructor. 2: econstructor.
-  2: { eexists. split. eauto. eauto. }
+  2: { eexists. split. eauto. eexists. eauto. }
   eexists. eauto.
-  eexists. split. eauto. eauto.
+  eexists. split. eexists. eauto. eauto.
 Qed.
 
 
@@ -207,14 +207,12 @@ Fixpoint val_type v T {struct T}: Prop :=
   match v, T with
   | vbool b, TBool =>  
       True
-  | vabs H ty, TFun T1' T2' =>
-      forall vx T1,
-        type_normalize T1 T1' ->
-        val_type vx T1' ->
-        exists vy T2,
+  | vabs H ty, TFun T1 T2 =>
+      forall vx,
+        val_type vx T1 ->
+        exists vy,
           tevaln (vx::H) ty vy /\
-          type_normalize T2 T2' /\
-          val_type vy T2'
+          val_type vy T2
   | _,_ =>
       False
   end.
@@ -256,11 +254,13 @@ Lemma type_eval_unique: forall T V1,
 Proof.
   intros T V1 H. induction H; intros.
   - inversion H. eauto.
-  - inversion H. eauto.
-  - inversion H1. subst. eapply IHtype_eval1 in H3. inversion H3. subst.
-    eauto.
-  - inversion H1. subst. eapply IHtype_eval1 in H3. inversion H3. subst.
-    eauto.
+  - inversion H1. subst. erewrite IHtype_eval1, IHtype_eval2; eauto.
+  - inversion H0. subst.
+    assert (TVFun V1 V2 = TVFun V0 V4). erewrite IHtype_eval; eauto.
+    inversion H1. eauto. 
+  - inversion H0. subst.
+    assert (TVFun V1 V2 = TVFun V3 V0). erewrite IHtype_eval; eauto.
+    inversion H1. eauto. 
 Qed.
 
 Lemma type_reify_unique: forall T V1,
@@ -270,13 +270,7 @@ Lemma type_reify_unique: forall T V1,
 Proof.
   intros T V1 H. induction H; intros.
   - inversion H. eauto.
-  - eapply IHtype_reify1 in H1. eapply IHtype_reify2 in H2. subst.
-    inversion H3. subst.
-    assert (V1 = V3). eapply type_eval_unique; eauto.
-    assert (V2 = V4). eapply type_eval_unique; eauto.
-    subst.
-    eapply IHtype_reify1 in H8. eapply IHtype_reify2 in H10. subst.
-    eauto. 
+  - inversion H1. subst. erewrite IHtype_reify1, IHtype_reify2; eauto. 
 Qed.
 
 Lemma type_normalize_unique: forall T V1,
@@ -362,7 +356,7 @@ Lemma sem_true: forall G,
     sem_type G ttrue TBool.
 Proof.
   intros. intros WFG. split. eexists. eauto. 
-  intros E WFE. exists (vbool true), TBool. split. 2: split. 
+  intros E WFE. exists (vbool true), TBool. split. 2: split.
   - exists 0. intros. destruct n. lia. simpl. eauto.
   - eauto.
   - simpl. eauto.
@@ -429,25 +423,22 @@ Proof.
     destruct WX as (TX' & VX & NX1 & NX2).
     destruct WF as (TF' & VF & NF1 & NF2).
     inversion NX1. subst.
-    assert (VF = TVFun T1 T2). eapply type_eval_unique; eauto. subst.
+    assert (VF = TVFun VX V2). eapply type_eval_unique; eauto. subst.
     inversion NF2. subst. 
     eexists _,_. split. econstructor; eauto. eauto.
   }
   split. eauto. intros E WFE.
-  (* TODO: eliminate some redundancy? *)
   destruct (HF E WFE) as (vf & TF' & STF & NF & VF).
   destruct (HX E WFE) as (vx & TX' & STX & NX & VX).
   destruct NF as (NF' & NF1 & NF2).
   destruct NX as (NX' & NX1 & NX2).
   inversion NX1. subst.
-  assert (NF' = TVFun T1 T2). eapply type_eval_unique; eauto. subst.
+  assert (NF' = TVFun NX' V2). eapply type_eval_unique; eauto. subst.
   destruct vf, TF'; simpl in VF; intuition.
   - inversion NF2. 
   - inversion NF2. subst.
-    assert (NX' = V1). eapply type_eval_unique; eauto. subst. 
-    assert (TF'1 = TX'). eapply type_reify_unique; eauto. subst. 
-    edestruct VF as (vy & T2'' & STY & NY & VY).
-    eexists. split. 2: eauto. eauto. eauto.
+    assert (TF'1 = TX'). eapply type_reify_unique; eauto. subst.
+    edestruct VF as (vy & STY & VY). eauto. 
     exists vy. exists TF'2. split. 2: split. 
     + destruct STF as (n1 & STF).
       destruct STX as (n2 & STX).
@@ -479,7 +470,7 @@ Proof.
   - simpl. intros.
     edestruct HY as (vy & TY' & ? & ? & ?). eapply envt_extend; eauto.
     assert (TY' = T2'). eapply type_normalize_unique; eauto.
-    subst. eexists _,_. eauto. 
+    subst. exists vy. eauto. 
 Qed.
 
 Lemma sem_equiv: forall G t T1 T2,
@@ -491,8 +482,8 @@ Proof.
   destruct H as (W1 & H). eauto. 
   destruct H0 as (T' & N1 & N2).
   split. eexists. eauto. intros E WFE.
-  edestruct H as (v & T1' & ? & ? & ?). eauto.
-  assert (T1' = T'). eapply type_normalize_unique; eauto. 
+  edestruct H as (v & T1'' & ? & ? & ?). eauto.
+  assert (T1'' = T'). eapply type_normalize_unique; eauto.
   subst. eexists _,_. split. 2: split.
   - eauto.
   - eauto.
